rt riscv ainvs: prove RISCV64 version of AInvs
Signed-off-by: Gerwin Klein <gerwin.klein@data61.csiro.au>

spec/haskell/src/SEL4/Object/CNode.lhs
@@ -338,7 +338,7 @@ Determine whether the CTE is valid, and has children to be deleted. If a child i
 >         nextCTE <- withoutPreemption $ getCTE nextPtr
 >         when (cte `isMDBParentOf` nextCTE) $ do
 >             cteDelete nextPtr True
->             preemptionPoint
+>
 >             cteRevoke slot
 
 \subsubsection{Deleting Capabilities}
