proof/invariant-abstract/RISCV64/ArchCSpaceInv_AI.thy
@@ -81,50 +81,18 @@ lemma replace_cap_invs:
     apply (clarsimp simp: irq_revocable_def)
    apply clarsimp
    apply (clarsimp simp: irq_revocable_def)
-  apply (rule conjI)
-   apply (erule disjE)
-    apply (simp add: fun_upd_def[symmetric] fun_upd_idem)
-   apply (simp add: reply_master_revocable_def)
-  apply (rule conjI)
-   apply (erule disjE)
-    apply (simp add: fun_upd_def[symmetric] fun_upd_idem)
-   apply (clarsimp simp add: reply_mdb_def)
-   apply (thin_tac "\<forall>a b. (a, b) \<in> cte_refs cp nd \<and> Q a b\<longrightarrow> R a b" for cp nd Q R)
-   apply (thin_tac "is_pt_cap cap \<longrightarrow> P" for cap P)+
-   apply (rule conjI)
-    apply (unfold reply_caps_mdb_def)[1]
-    apply (erule allEI, erule allEI)
-    apply (clarsimp split: if_split simp add: is_cap_simps
-                 simp del: split_paired_Ex split_paired_All)
-    apply (rename_tac ptra ptrb rights')
-    apply (rule_tac x="(ptra,ptrb)" in exI)
-    apply fastforce
-   apply (unfold reply_masters_mdb_def)[1]
-   apply (erule allEI, erule allEI)
-   subgoal by (fastforce split: if_split_asm simp: is_cap_simps)
-  apply (rule conjI)
-   apply (erule disjE)
-    apply (clarsimp simp add: is_reply_cap_to_def)
-    apply (drule caps_of_state_cteD)
-    apply (subgoal_tac "cte_wp_at (is_reply_cap_to t) p s")
-     apply (erule(1) valid_reply_capsD [OF has_reply_cap_cte_wpD])
-    apply (erule cte_wp_at_lift)
-    apply (fastforce simp add:is_reply_cap_to_def)
-   apply (simp add: is_cap_simps)
   apply (frule(1) valid_global_refsD2)
   apply (frule(1) cap_refs_in_kernel_windowD)
   apply (rule conjI)
-   apply (erule disjE)
-    apply (clarsimp simp: valid_reply_masters_def cte_wp_at_caps_of_state)
-    apply (cases p, fastforce simp:is_master_reply_cap_to_def)
-   apply (simp add: is_cap_simps)
-  apply (elim disjE)
-   apply simp
+   apply (erule disjE; simp add: is_cap_simps)
+  apply (erule disjE)
    apply (clarsimp simp: valid_table_capsD[OF caps_of_state_cteD]
-                    valid_arch_caps_def unique_table_refs_no_cap_asidE)
-  apply (rule conjI, clarsimp)
-  apply (rule conjI, rule Ball_emptyI, simp add: gen_obj_refs_subset)
-  by clarsimp
+                         valid_arch_caps_def unique_table_refs_no_cap_asidE)
+  apply (rule conjI)
+   apply (rule Ball_emptyI, simp add: gen_obj_refs_subset)
+  apply (clarsimp simp: valid_table_capsD[OF caps_of_state_cteD]
+                        valid_arch_caps_def unique_table_refs_no_cap_asidE)
+  done
 
 definition
   "is_simple_cap_arch cap \<equiv> \<not>is_pt_cap cap"
