proof/invariant-abstract/RISCV64/ArchDetSchedDomainTime_AI.thy
@@ -18,46 +18,53 @@ crunch domain_list_inv [wp, DetSchedDomainTime_AI_assms]: arch_finalise_cap "\<l
 crunch domain_list_inv [wp, DetSchedDomainTime_AI_assms]:
   arch_activate_idle_thread, arch_switch_to_thread, arch_switch_to_idle_thread,
   handle_arch_fault_reply,
-  arch_invoke_irq_control, arch_get_sanitise_register_info,
-  prepare_thread_delete, handle_hypervisor_fault, make_arch_fault_msg,
-  arch_post_modify_registers, arch_post_cap_deletion, handle_vm_fault,
-  arch_invoke_irq_handler
-  "\<lambda>s. P (domain_list s)"
-  (simp: crunch_simps)
+  arch_invoke_irq_control, handle_vm_fault, arch_get_sanitise_register_info,
+  prepare_thread_delete, handle_hypervisor_fault, make_arch_fault_msg,init_arch_objects,
+  arch_post_modify_registers, arch_post_cap_deletion, arch_invoke_irq_handler
+  "\<lambda>s::det_state. P (domain_list s)"
+  (wp: crunch_wps)
 
 crunch domain_time_inv [wp, DetSchedDomainTime_AI_assms]: arch_finalise_cap "\<lambda>s. P (domain_time s)"
-  (wp: hoare_drop_imps mapM_wp subset_refl simp: crunch_simps)
+  (wp: crunch_wps simp: crunch_simps)
 
 crunch domain_time_inv [wp, DetSchedDomainTime_AI_assms]:
   arch_activate_idle_thread, arch_switch_to_thread, arch_switch_to_idle_thread,
   handle_arch_fault_reply, init_arch_objects,
-  arch_invoke_irq_control, arch_get_sanitise_register_info,
-  prepare_thread_delete, handle_hypervisor_fault, handle_vm_fault,
-  arch_post_modify_registers, arch_post_cap_deletion, make_arch_fault_msg,
-  arch_invoke_irq_handler
-  "\<lambda>s. P (domain_time s)"
-  (simp: crunch_simps)
+  arch_invoke_irq_control, handle_vm_fault,
+  prepare_thread_delete, handle_hypervisor_fault,
+  arch_post_modify_registers, arch_post_cap_deletion, arch_invoke_irq_handler,
+  make_arch_fault_msg
+  "\<lambda>s::det_state. P (domain_time s)"
+  (wp: crunch_wps)
 
-crunches do_machine_op
-  for exst[wp]: "\<lambda>s. P (exst s)"
+crunches make_arch_fault_msg
+  for domain_consumed[DetSchedDomainTime_AI_assms]: "\<lambda>s. P (domain_time s) (consumed_time s)"
+  (wp: crunch_wps)
 
 declare init_arch_objects_exst[DetSchedDomainTime_AI_assms]
+        make_arch_fault_msg_invs[DetSchedDomainTime_AI_assms]
+        arch_get_sanitise_register_info_inv[DetSchedDomainTime_AI_assms]
+
+crunch domain_consumed_time_inv [wp, DetSchedDomainTime_AI_assms]:
+  arch_switch_to_idle_thread,arch_switch_to_thread "\<lambda>s. P (domain_time s)(consumed_time s)"
+  (simp: whenE_def)
 
 end
 
 global_interpretation DetSchedDomainTime_AI?: DetSchedDomainTime_AI
-  proof goal_cases
+proof goal_cases
   interpret Arch .
   case 1 show ?case by (unfold_locales; (fact DetSchedDomainTime_AI_assms)?)
-  qed
+qed
 
 context Arch begin global_naming RISCV64
 
-crunch domain_time_inv [wp, DetSchedDomainTime_AI_assms]: arch_perform_invocation "\<lambda>s. P (domain_time s)"
+crunches arch_perform_invocation, arch_mask_irq_signal
+  for domain_time_inv [wp, DetSchedDomainTime_AI_assms]: "\<lambda>s::det_state. P (domain_time s)"
+  and domain_list_inv [wp, DetSchedDomainTime_AI_assms]: "\<lambda>s::det_state. P (domain_list s)"
   (wp: crunch_wps check_cap_inv)
 
-crunch domain_list_inv [wp, DetSchedDomainTime_AI_assms]: arch_perform_invocation "\<lambda>s. P (domain_list s)"
-  (wp: crunch_wps check_cap_inv)
+crunch domain_time_sched[wp]: do_machine_op "\<lambda>s. P (domain_time s) (scheduler_action s)"
 
 lemma handle_interrupt_valid_domain_time [DetSchedDomainTime_AI_assms]:
   "\<lbrace>\<lambda>s :: det_ext state. 0 < domain_time s \<rbrace> handle_interrupt i
@@ -65,21 +72,21 @@ lemma handle_interrupt_valid_domain_time [DetSchedDomainTime_AI_assms]:
    apply (unfold handle_interrupt_def)
    apply (case_tac "maxIRQ < i"; simp)
     subgoal by (wp hoare_false_imp, simp)
-   apply (rule hoare_pre)
-    apply (wp do_machine_op_exst | simp add: arch_mask_irq_signal_def | wpc)+
+  apply (rule hoare_pre)
+    apply (wp  | simp add: arch_mask_irq_signal_def | wpc)+
        apply (rule_tac Q="\<lambda>_ s. 0 < domain_time s" in hoare_post_imp, fastforce)
        apply wp
       apply (rule_tac Q="\<lambda>_ s. 0 < domain_time s" in hoare_post_imp, fastforce)
       apply wp+
      apply simp (* dxo_eq *)
-     apply (clarsimp simp: timer_tick_def num_domains_def)
+     apply (clarsimp simp: num_domains_def)
      apply (wp reschedule_required_valid_domain_time
            | simp add: handle_reserved_irq_def
            | wp (once) hoare_drop_imp)+
     apply clarsimp
    done
 
-crunches handle_reserved_irq, arch_mask_irq_signal
+crunches handle_reserved_irq
   for domain_time_inv [wp, DetSchedDomainTime_AI_assms]: "\<lambda>s. P (domain_time s)"
   and domain_list_inv [wp, DetSchedDomainTime_AI_assms]: "\<lambda>s. P (domain_list s)"
   (wp: crunch_wps mapM_wp subset_refl simp: crunch_simps)
@@ -87,9 +94,9 @@ crunches handle_reserved_irq, arch_mask_irq_signal
 end
 
 global_interpretation DetSchedDomainTime_AI_2?: DetSchedDomainTime_AI_2
-  proof goal_cases
+proof goal_cases
   interpret Arch .
   case 1 show ?case by (unfold_locales; (fact DetSchedDomainTime_AI_assms)?)
-  qed
+qed
 
 end
