proof/invariant-abstract/RISCV64/ArchSyscall_AI.thy
@@ -17,8 +17,8 @@ context Arch begin global_naming RISCV64
 
 named_theorems Syscall_AI_assms
 
-declare arch_get_sanitise_register_info_invs[Syscall_AI_assms]
-crunch pred_tcb_at[wp,Syscall_AI_assms]: handle_arch_fault_reply, arch_get_sanitise_register_info "pred_tcb_at proj P t"
+declare arch_get_sanitise_register_info_inv[Syscall_AI_assms]
+crunch pred_tcb_at[wp,Syscall_AI_assms]: handle_arch_fault_reply, arch_get_sanitise_register_info "\<lambda>s. N (pred_tcb_at proj P t s)"
 crunch invs[wp,Syscall_AI_assms]: handle_arch_fault_reply "invs"
 crunch cap_to[wp,Syscall_AI_assms]: handle_arch_fault_reply, arch_get_sanitise_register_info "ex_nonz_cap_to c"
 crunch it[wp,Syscall_AI_assms]: handle_arch_fault_reply, arch_get_sanitise_register_info "\<lambda>s. P (idle_thread s)"
@@ -67,16 +67,14 @@ lemma handle_vm_fault_valid_fault[wp, Syscall_AI_assms]:
    apply (wp | simp add: valid_fault_def)+
   done
 
-
-lemma hvmf_active [Syscall_AI_assms]:
-  "\<lbrace>st_tcb_at active t\<rbrace> handle_vm_fault t w \<lbrace>\<lambda>rv. st_tcb_at active t\<rbrace>"
-  unfolding handle_vm_fault_def by (cases w; wpsimp)
+lemma hvmf_st_tcb_at[wp, Syscall_AI_assms]:
+  "handle_vm_fault t w \<lbrace>\<lambda>s. N (st_tcb_at P t' s)\<rbrace>"
+  unfolding handle_vm_fault_def
+  by (cases w; wpsimp)
 
 lemma hvmf_ex_cap[wp, Syscall_AI_assms]:
   "\<lbrace>ex_nonz_cap_to p\<rbrace> handle_vm_fault t b \<lbrace>\<lambda>rv. ex_nonz_cap_to p\<rbrace>"
   unfolding handle_vm_fault_def by (cases b; wpsimp)
-
-declare arch_get_sanitise_register_info_ex_nonz_cap_to[Syscall_AI_assms]
 
 lemma hh_invs[wp, Syscall_AI_assms]:
   "\<lbrace>invs and ct_active and st_tcb_at active thread and ex_nonz_cap_to_thread\<rbrace>
@@ -84,12 +82,16 @@ lemma hh_invs[wp, Syscall_AI_assms]:
    \<lbrace>\<lambda>rv. invs\<rbrace>"
   by (cases fault) wpsimp
 
+crunches make_fault_msg
+  for cur_sc[wp, Syscall_AI_assms]: "\<lambda>s. P (cur_sc s)"
+  and pred_tcb_at[wp, Syscall_AI_assms]: "pred_tcb_at proj P t"
+
 end
 
 global_interpretation Syscall_AI?: Syscall_AI
-  proof goal_cases
+proof goal_cases
   interpret Arch .
   case 1 show ?case by (unfold_locales; (fact Syscall_AI_assms)?)
-  qed
+qed
 
 end
